chore: make code compile

Veir/Data/PBV/Mask.lean
@@ -18,7 +18,7 @@ def maskOfWidth (o w : Nat) : BitVec o := BitVec.ofNat o (2 ^ w - 1)
 
 /-- `IsMask` encodes `m = 2^k - 1` for some `k : Nat` in terms of bitvector
 operations removing the dependency on `k` and allowing it to be bitblasted. -/
-def IsMask {o : Nat} (m : BitVec o) : Prop := m &&& (m + 1#o) = 0#o
+@[expose] def IsMask {o : Nat} (m : BitVec o) : Prop := m &&& (m + 1#o) = 0#o
 
 theorem toNat_maskOfWidth {o w : Nat} (h : w ≤ o) :
     (maskOfWidth o w).toNat = 2 ^ w - 1 := by
