Veir/Data/PBV/Examples.lean
@@ -75,6 +75,7 @@ theorem trace_double_zero_extend (p q r : Nat) (x : BitVec p)
   -- Translate the condition on the natural number width
   -- into a fact about the bitvector masks
   have le_pq := mask_lt_mask p_le_bw q_le_bw h_mp h_mq hpq
+  simp only [IsMask] at mr_mask mq_mask mp_mask
 -- Step 6:
   simp only [
     eq_iff r_le_bw,
@@ -122,11 +123,12 @@ theorem trace_zero_sign_extend (p q r : Nat) (x : BitVec p)
   -- Translate the condition on the natural number width
   -- into a fact about the bitvector masks
   have le_pq := mask_lt_mask p_le_bw q_le_bw h_mp h_mq hpq
+  simp only [IsMask] at mr_mask mq_mask mp_mask
 -- Step 6:
   simp only [
     eq_iff r_le_bw,
-    setWidth_signExtend r_le_bw,   -- Push `setWidth` down signExtend
-    msb_toMask q_le_bw,            -- Replace the sign bit test with a mask test
+    setWidth_signExtend_eq_and_maskOfWidth r_le_bw,  -- Push `setWidth` down signExtend
+    msb_eq_and_maskOfWidth_ne_zero q_le_bw,          -- Replace the sign bit test with a mask test
     setWidth_setWidth r_le_bw,
     setWidth_setWidth q_le_bw,
     setWidth_setWidth p_le_bw,
